WIP

src/Bedrock/Proofs/LoadStoreList.v
@@ -13,6 +13,7 @@ Require Import coqutil.Word.Interface coqutil.Word.Properties.
 Require Import coqutil.Map.Interface coqutil.Map.Properties.
 Require Import Crypto.Bedrock.Types.
 Require Import Crypto.Bedrock.Tactics.
+Require Import Crypto.Bedrock.Util.
 Require Import Crypto.Bedrock.Proofs.Dexprs.
 Require Import Crypto.Bedrock.Proofs.Flatten.
 Require Import Crypto.Bedrock.Proofs.Varnames.
@@ -41,21 +42,24 @@ Section LoadStoreList.
      (other values are ignored) *)
   Fixpoint lists_reserved {t}
     : base_list_lengths t ->
-      Semantics.mem -> (* memory *)
+      list_locs t ->
+      Semantics.mem ->
       Prop :=
-    match t with
+    match t as t0 return base_list_lengths t0 -> list_locs t0 -> _ with
     | base.type.prod a b =>
-      fun x => sep (lists_reserved (fst x)) (lists_reserved (snd x))
+      fun x y => sep (lists_reserved (fst x) (fst y))
+                            (lists_reserved (snd x) (snd y))
     | base_listZ =>
-      fun n =>
-        Lift1Prop.ex1
-          (fun start : Semantics.word =>
-             Lift1Prop.ex1
-               (fun oldvalues : list Semantics.word =>
-                  let size := Interface.word.of_Z (Z.of_nat n) in
-                  array scalar size start oldvalues))
-    | base_Z => fun _ _ => True
-    |  _ => fun _ _ => False
+      fun n loc =>
+        (Lift1Prop.ex1
+           (fun oldvalues : list Z =>
+              sep (map:=Semantics.mem)
+                  (emp (length oldvalues = n))
+                  (rep.equiv (rep:=rep.listZ_mem) oldvalues
+                             (expr.literal (word.unsigned loc))
+                             map.empty)))
+    | base_Z => fun _ _ => emp True
+    |  _ => fun _ _ => emp False
     end.
 
   Fixpoint list_lengths_from_value {t}
@@ -97,12 +101,7 @@ Section LoadStoreList.
                      rep.rtype_of_ltype rep.listZ_mem ]; intros.
     cbn [WeakestPrecondition.dexpr
            WeakestPrecondition.expr WeakestPrecondition.expr_body] in *.
-    repeat match goal with
-           | H : sep (Lift1Prop.ex1 _) _ _ |- _ =>
-             apply sep_ex1_l in H; destruct H; cbv zeta in *
-           | H : context [emp] |- _ =>
-             apply sep_assoc, sep_emp_l in H; cleanup
-           end.
+    sepsimpl.
     match goal with
     | H : context[array] |- _ =>
       eapply Proper_sep_iff1 in H;
@@ -255,17 +254,7 @@ Section LoadStoreList.
                flatten_base_ltype equivalent_flat_base
                base_rtype_of_ltype
                rep.varname_set rep.Z
-          ]; break_match; intros;
-        repeat match goal with
-                 | _ => progress cleanup
-                 | H : sep (sep (emp _) _) _ _ |- _ =>
-                   apply sep_assoc in H
-                 | H : sep (emp _) _ _ |- _ =>
-                   apply sep_emp_l in H
-                 | H : sep (Lift1Prop.ex1 _) _ _ |- _ =>
-                   apply sep_ex1_l in H; destruct H
-                 | H : False |- _ => tauto
-               end.
+          ]; break_match; intros; sepsimpl; [ | | ].
     { (* base_Z *)
       repeat straightline. cbv [emp].
       repeat match goal with
@@ -414,8 +403,7 @@ Section LoadStoreList.
           setoid_rewrite not_union_iff in H;
             apply H; lia
           end. }
-        {
-          match goal with
+        { match goal with
           | H : sep (sep ?p ?q) ?r ?m |- sep _ _ ?m =>
             apply sep_comm, sep_assoc, sep_comm in H;
             eapply Proper_sep_iff1; [ | reflexivity | apply H]
@@ -444,38 +432,387 @@ Section LoadStoreList.
             intros; cleanup. subst.
             eauto with lia. } } } }
     { (* arrow (arrow _ _) _ *)
-      match goal with
-      | H : sep (emp False) _ _ |- _ =>
-        eapply sep_emp_l in H; tauto
-      end. }
+      sepsimpl. }
   Qed.
 
-  (* idea: pull return list lengths from fiat-crypto type *)
+  (* TODO: move? *)
+  Lemma equiv_nil_iff1 y locals :
+    Lift1Prop.iff1
+      (rep.equiv (rep:=rep.listZ_mem) [] y locals)
+      (Lift1Prop.ex1
+         (fun x => rep.equiv (rep:=rep.Z) x y locals)).
+  Proof.
+    cbv [rep.equiv rep.listZ_mem rep.Z array map].
+    intro; split; intros;
+      repeat match goal with
+             | _ => progress subst
+             | _ => progress sepsimpl
+             | |- Lift1Prop.ex1 _ _ => eexists
+             | |- _ /\ _ => split
+             | _ => solve [eauto]
+             end.
+  Qed.
+
+  Lemma lists_reserved_0 loc:
+    Lift1Prop.iff1
+      (lists_reserved (t:=base_listZ) 0%nat loc)
+      (emp True).
+  Proof.
+    cbv [lists_reserved].
+    split; intros;
+      repeat match goal with
+             | _ => progress (sepsimpl; subst)
+             | H : Datatypes.length _ = 0%nat |- _ =>
+               apply length0_nil in H; subst
+             | H : rep.equiv _ _ _ _ |- _ => apply equiv_nil_iff1 in H
+             | H : rep.equiv _ (expr.literal _) _ _ |- _ =>
+               destruct H; subst
+             | |- Lift1Prop.ex1 _ _ => eexists
+             | |- _ /\ _ => split
+             | _ => solve [eauto using List.length_nil]
+             end.
+    apply equiv_nil_iff1.
+    eexists; eexists; reflexivity.
+  Qed.
+
+  (* TODO: move? *)
+  Lemma dexpr_equiv m l n x1 x2 :
+    WeakestPrecondition.dexpr m l (expr.var n) x1 ->
+    WeakestPrecondition.dexpr m l (expr.var n) x2 ->
+    x1 = x2.
+  Proof.
+    destruct 1; destruct 1; cleanup; congruence.
+  Qed.
+
+  Lemma store_list_correct :
+    forall (start : string)
+           (loc : list_locs base_listZ)
+           (functions : list _)
+           (value_names2 value_names1 : list string)
+           (rets1 rets2 rets : base.interp base_listZ)
+           (i : nat)
+           (tr : Semantics.trace)
+           (locals : Semantics.locals)
+           (mem : Semantics.mem)
+           (R : Semantics.mem -> Prop),
+      let retlengths :=
+          list_lengths_from_value (t:=base_listZ) rets2 in
+      let loc' :=
+          word.add loc (word.of_Z (Z.of_nat i * word_size_in_bytes)) in
+      let values1 := map expr.var value_names1 in
+      let values2 := map expr.var value_names2 in
+      rets = rets1 ++ rets2 ->
+      length rets1 = length value_names1 ->
+      length rets2 = length value_names2 ->
+      length value_names1 = i ->
+      sep (map:=Semantics.mem)
+          (rep.equiv (rep:=rep.Z) (word.unsigned loc) (expr.var start) locals)
+          (rep.equiv (rep:=rep.listZ_local) rets2 values2 locals) mem ->
+      (* use old values of memory to set up frame for return values *)
+      sep (map:=Semantics.mem)
+          (sep (map:=Semantics.mem)
+               (rep.equiv (rep:=rep.listZ_mem)
+                          rets1 (expr.var start) locals)
+               (lists_reserved retlengths loc')) R mem ->
+      WeakestPrecondition.cmd
+        (WeakestPrecondition.call functions)
+        (store_list (expr.var start) values2 i) tr mem locals
+        (fun tr' mem' locals' =>
+           tr = tr' /\
+           locals = locals' /\
+           sep (map:=Semantics.mem)
+               (rep.equiv (rep:=rep.listZ_mem)
+                          rets (expr.var start) locals') R mem').
+  Proof.
+    cbv zeta.
+    induction value_names2 as [|n0 ?]; destruct rets2 as [|r0 rets2];
+      cbn [store_list Datatypes.length
+                      rep.equiv rep.listZ_local rep.Z rep.listZ_mem];
+      intros; subst; try lia; sepsimpl.
+    { repeat split; try reflexivity.
+      repeat match goal with
+             | _ => progress sepsimpl
+             | H : _ |- _ =>
+               rewrite List.firstn_all, List.skipn_all_exact in H
+             | |- Lift1Prop.ex1 _ _ => eexists
+             | |- _ /\ _ => split
+             | _ => eassumption
+             end.
+      match goal with
+      | H: context [array] |- _ =>
+        refine (Lift1Prop.subrelation_iff1_impl1 _ _ _ _ _ H); clear H
+      end.
+      rewrite app_nil_r.
+      rewrite lists_reserved_0. cancel. }
+    { repeat match goal with
+             | H : _ |- _ => rewrite word.of_Z_unsigned in H end.
+      match goal with H1 : _, H2 : _ |- _ =>
+                      rewrite (dexpr_equiv _ _ _ _ _ H1 H2) in *;
+                        clear H1
+      end.
+      subst; eexists; split.
+      { cbn [WeakestPrecondition.dexpr
+               WeakestPrecondition.expr
+               WeakestPrecondition.expr_body] in *.
+        eapply Proper_get; [ | eassumption ].
+        repeat intro; subst.
+        reflexivity. }
+      cbn [map] in *.
+      match goal with
+      | H : Forall2 _ (_ :: _) (_ :: _) |- _ => inversion H; subst; clear H
+      end.
+      sepsimpl.
+      eexists; split.
+      { cbn [WeakestPrecondition.dexpr
+               WeakestPrecondition.expr
+               WeakestPrecondition.expr_body] in *.
+        eassumption. }
+      cbn [lists_reserved
+             list_lengths_from_value
+             rep.equiv rep.Z rep.listZ_mem] in *.
+      sepsimpl.
+      match goal with
+        H : Datatypes.length ?x = Datatypes.length (_ :: _) |- _ =>
+        destruct x; cbn [Datatypes.length] in H; [ lia | ]
+      end.
+      cbn [map array Semantics.interp_binop] in *.
+      eapply store_word_of_sep.
+      { cbn [WeakestPrecondition.dexpr
+               WeakestPrecondition.expr
+               WeakestPrecondition.expr_body] in *.
+        cbv [WeakestPrecondition.literal dlet.dlet] in *.
+        match goal with H : word.of_Z _ = word.of_Z _ |- _ =>
+                        rewrite ?word.of_Z_unsigned in H;
+                          rewrite H in * end.
+        ecancel_assumption. }
+      intros. sepsimpl.
+      eapply Proper_cmd; [ solve [apply Proper_call] | repeat intro | ].
+      2:{
+        eapply IHvalue_names2 with
+            (rets1:= rets1 ++ [r0]) (rets2:=rets2)
+            (value_names1:=value_names1 ++ [n0]);
+        rewrite ?app_length; cbn [length]; eauto; try lia; [ | ].
+        { rewrite word.of_Z_unsigned.
+          cbn [rep.equiv rep.Z rep.listZ_local].
+          sepsimpl; eauto using Forall.Forall2_skipn. }
+        {
+          (* look at goal and plug in evars very carefully *)
+          sepsimpl.
+          match goal with H: ?P (expr.var start) (word.of_Z ?x) |- _ =>
+                          exists x end.
+          sepsimpl; auto.
+          match goal with
+            H : context [array _ _ (word.add _ _) (map _ ?x)] |- _ =>
+            exists x end.
+          sepsimpl; auto.
+          eexists; sepsimpl; try reflexivity.
+          match goal with
+            H : context [array _ _ (word.add (word.add _ _) _) _] |- _ =>
+            refine (Lift1Prop.subrelation_iff1_impl1 _ _ _ _ _ H); clear H
+          end.
+          rewrite map_app, array_append. cbn [map array].
+          match goal with
+            |- context [word.add (word.add ?a (word.of_Z (Z.of_nat ?b * ?c))) (word.of_Z ?c)] =>
+            replace (word.add (word.add a (word.of_Z (Z.of_nat b * c))) (word.of_Z c)) with
+              (word.add a (word.of_Z (Z.of_nat (S b) * c)))
+              by (apply word.unsigned_inj;
+                  rewrite Nat2Z.inj_succ, <-Z.add_1_r;
+                  rewrite !word.unsigned_add, !word.unsigned_of_Z;
+                  cbv [word.wrap]; Modulo.pull_Zmod; f_equal; lia)
+          end.
+          cbn [Compilers.base_interp] in *. (* simplifies implicit types *)
+          rewrite !word.of_Z_unsigned, ?map_length.
+          match goal with
+          | |- Lift1Prop.iff1 ?L ?R =>
+            let la := match L with context [scalar ?la] => la end in
+            let ra := match R with context [scalar ?ra] => ra end in
+            replace ra with la
+              by (apply word.unsigned_inj;
+                  rewrite !word.unsigned_add, !word.unsigned_of_Z;
+                  cbv [word.wrap]; Modulo.pull_Zmod; f_equal; lia)
+          end.
+          cancel. } }
+      cbv beta in *; cleanup; subst.
+      repeat match goal with |- _ /\ _ => split end;
+        eauto.
+      rewrite app_cons_app_app.
+      eassumption. }
+  Qed.
+
+  (* TODO: move *)
+  Lemma dexpr_put_same m l n x :
+    WeakestPrecondition.dexpr m (map.put l n x) (expr.var n) x.
+  Proof. eexists; rewrite map.get_put_same; tauto. Qed.
+
+  (* TODO: move *)
+  Lemma dexpr_put_diff m l n1 n2 x y :
+    n1 <> n2 ->
+    WeakestPrecondition.dexpr m l (expr.var n1) x ->
+    WeakestPrecondition.dexpr m (map.put l n2 y) (expr.var n1) x.
+  Proof.
+    destruct 2; intros; eexists; rewrite map.get_put_diff; eauto.
+  Qed.
+
+  (* TODO: move *)
+  Lemma Forall2_impl_strong {A B} (R1 R2 : A -> B -> Prop) xs ys :
+    (forall x y, R1 x y -> In x xs -> In y ys -> R2 x y) ->
+    Forall2 R1 xs ys -> Forall2 R2 xs ys.
+  Proof.
+    revert ys; induction xs; destruct ys; intros;
+      match goal with H : Forall2 _ _ _ |- _ =>
+                      inversion H; subst; clear H end;
+      constructor; eauto using in_eq, in_cons.
+  Qed.
+
+  (* TODO: move *)
+  Lemma varname_set_local x :
+    PropSet.sameset
+      (rep.varname_set (rep:=rep.listZ_local) x)
+      (PropSet.of_list x).
+  Proof.
+    apply sameset_iff.
+    cbn [rep.varname_set rep.listZ_local rep.Z].
+    induction x; cbn [fold_right PropSet.of_list In];
+      [ solve [firstorder idtac] | ].
+    intros. cbv [PropSet.of_list] in *.
+    rewrite <-IHx. firstorder idtac.
+  Qed.
+
   Lemma store_return_values_correct {t} :
     forall (retnames_local : base_ltype t)
            (retnames_mem : base_ltype t)
-           (retlengths : base_list_lengths t)
            (rets : base.interp t)
+           (locs : list_locs t)
            (functions : list _)
            (tr : Semantics.trace)
            (locals : Semantics.locals)
            (mem : Semantics.mem)
            (R : Semantics.mem -> Prop),
-        (* use old values of memory to set up frame for return values *)
-        sep (lists_reserved retlengths) R mem ->
-        (* rets are stored in local retnames *)
-        locally_equivalent
-          rets (base_rtype_of_ltype retnames_local) locals ->
-        (* translated function produces equivalent results *)
-        WeakestPrecondition.cmd
-          (WeakestPrecondition.call functions)
-          (store_return_values retnames_local retnames_mem)
-          tr mem locals
-          (fun tr' mem' locals' =>
-             tr = tr' /\
-             sep (equivalent
-                    rets (base_rtype_of_ltype retnames_mem) locals')
-                 R mem').
+      let retlengths := list_lengths_from_value rets in
+      (* use old values of memory to set up frame for return values *)
+      sep (lists_reserved retlengths locs) R mem ->
+      (* rets are stored in local retnames *)
+      locally_equivalent
+        rets (base_rtype_of_ltype retnames_local) locals ->
+      (* retnames are disjoint *)
+      PropSet.disjoint (varname_set retnames_local)
+                       (varname_set retnames_mem) ->
+      (* retnames don't contain duplicates *)
+      NoDup (flatten_base_ltype retnames_mem) ->
+      (* translated function produces equivalent results *)
+      WeakestPrecondition.cmd
+        (WeakestPrecondition.call functions)
+        (store_return_values retnames_local retnames_mem locs)
+        tr mem locals
+        (fun tr' mem' locals' =>
+           tr = tr' /\
+           map.only_differ locals (varname_set retnames_mem) locals' /\
+           sep (equivalent
+                  rets (base_rtype_of_ltype retnames_mem) locals')
+               R mem').
   Proof.
-  Admitted.
+    cbv zeta.
+    induction t;
+      cbn [fst snd store_return_values lists_reserved
+               locally_equivalent equivalent varname_set
+               base_rtype_of_ltype rep.rtype_of_ltype
+               rep.equiv rep.varname_set rep.Z
+               flatten_base_ltype list_lengths_from_value
+          ]; break_match; intros; sepsimpl; [ | | ].
+    { (* base_Z *)
+      repeat straightline.
+      eexists; split; [eassumption|].
+      cbv [dlet.dlet]; split; [reflexivity|].
+      split;
+        [ solve [eauto using only_differ_sym, only_differ_put] | ].
+      apply sep_emp_l. split; [|assumption].
+      cbv [WeakestPrecondition.dexpr
+             WeakestPrecondition.expr
+             WeakestPrecondition.expr_body
+             WeakestPrecondition.get] in *.
+      cleanup; subst. eexists.
+      rewrite map.get_put_same.
+      split; reflexivity. }
+    { (* prod *)
+      repeat straightline.
+      match goal with H : _ |- _ =>
+                      pose proof H;
+                      apply NoDup_app_iff in H; cleanup end.
+      repeat match goal with
+             | _ => progress cleanup
+             | H : PropSet.disjoint (PropSet.union _ _) _ |- _ =>
+               apply disjoint_union_l_iff in H
+             | H : PropSet.disjoint _ (PropSet.union _ _) |- _ =>
+               apply disjoint_union_r_iff in H
+             end.
+      eapply Proper_cmd;
+        [ solve [apply Proper_call] | repeat intro
+          | eapply IHt1; try ecancel_assumption; solve [eauto] ].
+      cbv beta in *. cleanup; subst.
+      eapply Proper_cmd;
+        [ solve [apply Proper_call] | repeat intro | ].
+      2:{ eapply IHt2; try ecancel_assumption; eauto.
+          cbv [locally_equivalent].
+          eapply equivalent_only_differ; eauto with equiv.
+          symmetry; eauto. }
+      cbv beta in *. cleanup; subst.
+      repeat match goal with |- _ /\ _ => split end;
+        eauto using only_differ_sym, only_differ_trans.
+      use_sep_assumption. cancel.
+      eapply equivalent_only_differ_iff1; eauto with equiv.
+      rewrite !varname_set_flatten.
+      symmetry.
+      eapply NoDup_disjoint; eauto using string_dec. }
+    { (* base_listZ *)
+      repeat straightline.
+      repeat match goal with p := _ |- _ => subst p end.
+      eapply Proper_cmd;
+        [ solve [apply Proper_call] | repeat intro | ].
+      2:{
+        eapply store_list_correct with
+            (rets:=rets) (rets1:=[]) (rets2:=rets)
+            (value_names1:=nil); auto using List.length_nil; [ | | ].
+        { cbn [rep.equiv rep.rtype_of_ltype rep.listZ_local] in *.
+          eapply Forall.eq_length_Forall2, Forall.Forall2_map_r_iff.
+          eauto. }
+        { cbn [rep.equiv rep.Z rep.rtype_of_ltype rep.listZ_local] in *.
+          sepsimpl; eauto using dexpr_put_same.
+          eapply Forall2_impl_strong; eauto.
+          intros; sepsimpl.
+          match goal with H : _ |- _ => apply in_map_iff in H end.
+          cleanup; subst.
+
+          cbn [rep.varname_set rep.listZ_mem rep.Z] in *.
+          match goal with H : _ |- _ =>
+                          rewrite varname_set_local in H end.
+          match goal with H : PropSet.disjoint _ _ |- _ =>
+                          apply disjoint_singleton_r_iff in H;
+                            eauto using string_dec;
+                            cbv [PropSet.of_list] in H
+          end.
+          apply dexpr_put_diff; [ | eassumption].
+          intro; subst; tauto. }
+        { apply sep_assoc.
+          eapply Proper_sep_iff1;
+            [ apply equiv_nil_iff1 | reflexivity | ].
+          sepsimpl. eexists.
+          apply sep_emp_l; split;
+            [ solve [eauto using dexpr_put_same] | ].
+          cbn [lists_reserved].
+          sepsimpl. eexists.
+          sepsimpl; eauto.
+          match goal with
+            |- context [word.unsigned (word.add ?x ?y)] =>
+            replace (word.unsigned (word.add x y)) with (word.unsigned x)
+          end; [ eassumption | ].
+          rewrite word.unsigned_add, word.unsigned_of_Z.
+          cbv [word.wrap].
+          rewrite Nat2Z.inj_0, Z.mul_0_l, Z.mod_0_l, Z.add_0_r
+            by eauto using Z.pow_nonzero, Z.lt_le_incl, word.width_pos with lia.
+          rewrite Z.mod_small by apply word.unsigned_range.
+          reflexivity. } }
+      cbv beta in *. cleanup; subst.
+      repeat match goal with |- _ /\ _ => split end;
+        eauto using only_differ_sym, only_differ_put. }
+  Qed.
 End LoadStoreList.
