src/Bedrock/Proofs/Varnames.v
@@ -1,8 +1,6 @@
 Require Import Coq.ZArith.ZArith.
 Require Import Coq.Strings.String.
 Require Import Coq.micromega.Lia.
-Require Import Coq.Classes.Morphisms.
-Require Import Coq.Classes.RelationClasses.
 Require Import bedrock2.Syntax.
 Require Import bedrock2.Map.Separation.
 Require Import bedrock2.Map.SeparationLogic.
@@ -12,6 +10,7 @@ Require Import coqutil.Datatypes.PropSet.
 Require Import Coq.Lists.List. (* after SeparationLogic *)
 Require Import Crypto.Bedrock.Types.
 Require Import Crypto.Bedrock.Tactics.
+Require Import Crypto.Bedrock.Util.
 Require Import Crypto.Language.API.
 Require Import Crypto.Util.ListUtil.
 Require Import Crypto.Util.Tactics.DestructHead.
@@ -21,187 +20,8 @@ Require Import Crypto.BoundsPipeline.
 
 Import API.Compilers.
 Import Wf.Compilers.expr.
+Import ListNotations.
 Import Types.Notations Types.Types.
-
-(* General-purpose lemmas about maps that should be later moved to coqutil *)
-(* TODO: move *)
-Section Sets.
-  Context {E : Type}.
-
-  Lemma disjoint_union_l_iff (s1 s2 s3 : set E) :
-    disjoint (union s1 s2) s3 <-> disjoint s1 s3 /\ disjoint s2 s3.
-  Proof. firstorder idtac. Qed.
-
-  Lemma disjoint_union_r_iff (s1 s2 s3 : set E) :
-    disjoint s1 (union s2 s3) <-> disjoint s1 s2 /\ disjoint s1 s3.
-  Proof. firstorder idtac. Qed.
-
-  Lemma disjoint_cons (s : set E) x l :
-    disjoint s (of_list (x :: l)) ->
-    disjoint s (of_list l) /\ disjoint s (singleton_set x).
-  Proof. firstorder idtac. Qed.
-
-  Lemma disjoint_singleton_r_iff
-        (x : E) (s : set E)
-        (eq_dec : forall a b : E, {a = b} + {a <> b}):
-    ~ s x <->
-    disjoint s (singleton_set x).
-  Proof.
-    intros. split; [|firstorder idtac].
-    intros. intro y.
-    destruct (eq_dec x y);
-      subst; try firstorder idtac.
-  Qed.
-
-  Lemma disjoint_singleton_singleton
-        (x y : E)
-        (eq_dec : forall a b : E, {a = b} + {a <> b}):
-    y <> x ->
-    disjoint (singleton_set x) (singleton_set y).
-  Proof.
-    intros.
-    apply disjoint_singleton_r_iff;
-      firstorder congruence.
-  Qed.
-
-  Lemma disjoint_sameset (s1 s2 s3 : set E) :
-    sameset s3 s1 ->
-    disjoint s1 s2 ->
-    disjoint s3 s2.
-  Proof. firstorder idtac. Qed.
-
-  Global Instance disjoint_sym : Symmetric (@disjoint E).
-  Proof. firstorder idtac. Defined.
-  Global Instance disjoint_Proper
-    : Proper (sameset ==> sameset ==> iff) (@disjoint E).
-  Proof. firstorder idtac. Defined.
-
-  Global Instance sameset_sym : Symmetric (@sameset E).
-  Proof. firstorder idtac. Defined.
-  Global Instance sameset_trans : Transitive (@sameset E).
-  Proof. firstorder idtac. Defined.
-  Global Instance sameset_ref : Reflexive (@sameset E).
-  Proof. firstorder idtac. Defined.
-
-  Lemma sameset_iff (s1 s2 : set E) :
-    sameset s1 s2 <-> (forall e, s1 e <-> s2 e).
-  Proof. firstorder idtac. Qed.
-
-  Lemma not_union_iff (s1 s2 : set E) x :
-    ~ union s1 s2 x <-> ~ s1 x /\ ~ s2 x.
-  Proof. firstorder idtac. Qed.
-End Sets.
-
-(* General-purpose lemmas about maps that should be later moved to coqutil *)
-(* TODO: move *)
-Section Maps.
-  Context {key value} {key_eqb}
-          {map : map.map key value}
-          {key_eq_dec :
-             forall x y : key,
-               BoolSpec (x = y) (x <> y) (key_eqb x y)}
-          {map_ok : map.ok map}.
-
-  Lemma only_differ_trans m1 m2 m3 ks1 ks2 :
-    map.only_differ m2 ks1 m1 ->
-    map.only_differ m3 ks2 m2 ->
-    map.only_differ m3 (union ks1 ks2) m1.
-  Proof.
-    (* TODO: map_solver should help with these but fails *)
-    (* 
-       Require Import coqutil.Map.Solver.
-       map_solver map_ok.
-    *)
-  Admitted.
-
-  Lemma only_differ_sym m1 m2 ks :
-    map.only_differ m2 ks m1 ->
-    map.only_differ m1 ks m2.
-  Admitted.
-
-  Lemma only_differ_sameset m1 m2 ks1 ks2 :
-    sameset ks1 ks2 ->
-    map.only_differ m2 ks1 m1 ->
-    map.only_differ m2 ks2 m1.
-  Admitted.
-
-  Lemma only_differ_put m k v :
-    map.only_differ (map.put m k v) (singleton_set k) m.
-  Admitted.
-
-  Lemma putmany_of_list_zip_app_l m ks1 ks2 vs :
-    map.putmany_of_list_zip (ks1 ++ ks2) vs m =
-    Option.bind
-      (map.putmany_of_list_zip
-         ks1 (List.firstn (Datatypes.length ks1) vs) m)
-      (map.putmany_of_list_zip
-         ks2 (List.skipn (Datatypes.length ks1) vs)).
-  Admitted.
-
-  Lemma putmany_of_list_zip_bind_comm m ks1 ks2 vs1 vs2 :
-    Option.bind
-      (map.putmany_of_list_zip ks1 vs1 m)
-      (map.putmany_of_list_zip ks2 vs2) =
-    Option.bind
-      (map.putmany_of_list_zip ks2 vs2 m)
-      (map.putmany_of_list_zip ks1 vs1).
-  Admitted.
-End Maps.
-
-(* General-purpose lemmas about lists that should be later moved to coqutil *)
-(* TODO: move *)
-Section Lists.
-  Context {A : Type}.
-
-  Lemma hd_map {B} (f : A -> B) x l :
-    hd (f x) (map f l) = f (hd x l).
-  Proof. destruct l; reflexivity. Qed.
-
-  Lemma hd_skipn_nth_default (d:A) l i :
-    nth_default d l i = hd d (skipn i l).
-  Proof.
-    revert i; induction l; destruct i; try reflexivity.
-    rewrite nth_default_cons_S, skipn_cons_S. eauto.
-  Qed.
-
-  Lemma firstn_length_firstn n (l : list A) :
-    firstn (length (firstn n l)) l = firstn n l.
-  Proof.
-    revert l; induction n; destruct l;
-      cbn [firstn length]; rewrite ?IHn; reflexivity.
-  Qed.
- 
-  Lemma skipn_length_firstn n (l : list A) :
-    skipn (length (firstn n l)) l = skipn n l.
-  Proof.
-    revert l; induction n; destruct l;
-      cbn [skipn firstn length]; rewrite ?IHn; reflexivity.
-  Qed.
-End Lists.
-
-(* General-purpose lemmas about sep that should be later moved to bedrock2 *)
-(* TODO: move *)
-Section Separation.
-  Context `{map_ok : map.ok}
-           {key_eqb : forall H H0 : key, bool}
-           {key_eq_dec :
-              forall x y : key,
-                BoolSpec (x = y) (x <> y) (key_eqb x y)}.
-  Lemma sep_empty_iff (q r : map.rep -> Prop) :
-    sep q r map.empty <-> q map.empty /\ r map.empty.
-  Proof.
-    cbv [sep].
-    repeat match goal with
-           | _ => progress (intros; cleanup)
-           | _ => progress subst
-           | H : _ |- _ => apply map.split_empty in H
-           | _ => rewrite map.split_empty
-           | _ => exists map.empty
-           | _ => tauto
-           | _ => split
-           end.
-  Qed.
-End Separation.
 
 (* Reasoning about various collections of variable names *)
 Section Varnames.
@@ -487,9 +307,10 @@ Section Varnames.
     map.only_differ l1 (used_varnames nextn (S nvars)) l2.
   Proof.
     intros.
-    eapply only_differ_sameset;
-    [ | eapply only_differ_trans;
-        eauto using only_differ_sym, only_differ_put ].
+    eapply Proper_only_differ;
+      [ reflexivity | | reflexivity
+        | eapply only_differ_trans;
+          solve [eauto using only_differ_sym, only_differ_put] ].
     eapply sameset_iff; intros.
     cbv [used_varnames of_list elem_of union singleton_set].
     cbn [seq map In].
