src/Bedrock/Tactics.v
@@ -1,4 +1,7 @@
 Require Import bedrock2.WeakestPreconditionProperties.
+Require Import bedrock2.Map.Separation bedrock2.Map.SeparationLogic.
+Require Import coqutil.Map.Interface.
+Require Import Crypto.Bedrock.Util.
 Require Import Crypto.Util.Tactics.DestructHead.
 Require Import Crypto.Util.Tactics.BreakMatch.
 Require Import Rewriter.Language.Wf.
@@ -72,3 +75,62 @@ Ltac peel_expr :=
                      destruct H as [? [_ [_ H] ] ]
                    end
                  end).
+
+Ltac sepsimpl_step' :=
+  match goal with
+  | |- sep (emp _) _ _ => apply sep_emp_l
+  | |- sep _ (emp _) _ => apply sep_emp_r
+  | |- sep (fun m => emp _ m) _ _ => apply sep_emp_l
+  | |- sep _ (fun m => emp _ m) _ => apply sep_emp_r
+  | |- sep (Lift1Prop.ex1 _) _ _ => apply sep_ex1_l
+  | |- sep _ (Lift1Prop.ex1 _) _ => apply sep_ex1_r
+  | |- emp _ _ => split; [ congruence | ]
+  end.
+
+Ltac sepsimpl_step :=
+  match goal with
+  | _ => sepsimpl_step'
+  | |- sep (sep _ _) _ _ => apply sep_assoc; sepsimpl_step'
+  | |- sep _ (sep _ _) _ => apply sep_comm, sep_assoc; sepsimpl_step'
+  | |- sep _ _ _ => apply sep_comm; sepsimpl_step'
+  end.
+
+Ltac sepsimpl_in H :=
+  match type of H with
+  | sep (emp _) _ _ =>
+    eapply sep_emp_l in H
+  | sep _ (emp _) _ =>
+    eapply sep_emp_r in H
+  | sep (fun m => emp _ m) _ _ =>
+    eapply sep_emp_l in H
+  | sep _ (fun m => emp _ m) _ =>
+    eapply sep_emp_r in H
+  | sep (Lift1Prop.ex1 _) _ _ =>
+    eapply sep_ex1_l in H; destruct H
+  | sep _ (Lift1Prop.ex1 _) _ =>
+    eapply sep_ex1_r in H; destruct H
+  | sep _ _ map.empty =>
+    apply sep_empty_iff in H
+  end.
+
+Ltac sepsimpl_hyps_step :=
+  match goal with
+  | H : False |- _ => tauto
+  | H : emp _ _ |- _ => cbv [emp] in H; destruct H
+  | H : Lift1Prop.ex1 _ _ |- _ => destruct H
+  | H : sep (sep ?p ?q) _ _ |- _ =>
+    eapply (sep_assoc p q) in H; sepsimpl_in H
+  | H : sep _ _ _ |- _ => sepsimpl_in H
+  | H : sep _ (sep ?p ?q) _ |- _ =>
+    eapply sep_comm, (sep_assoc p q) in H; sepsimpl_in H
+  end.
+
+Ltac sepsimpl_hyps :=
+  repeat first [ progress cleanup
+               | progress sepsimpl_hyps_step ].
+
+Ltac sepsimpl :=
+  repeat first [ progress cleanup
+               | match goal with |- _ /\ _ => split end
+               | progress sepsimpl_step
+               | progress sepsimpl_hyps_step ].
