src/Bedrock/Util.v
@@ -1,0 +1,249 @@
+Require Import Coq.ZArith.ZArith.
+Require Import Coq.Strings.String.
+Require Import Coq.micromega.Lia.
+Require Import Coq.Classes.Morphisms.
+Require Import Coq.Classes.RelationClasses.
+Require Import bedrock2.Syntax.
+Require Import bedrock2.Map.Separation.
+Require Import bedrock2.Map.SeparationLogic.
+Require Import coqutil.Tactics.destr.
+Require Import coqutil.Map.Interface coqutil.Map.Properties.
+Require Import coqutil.Word.Interface.
+Require Import coqutil.Datatypes.PropSet.
+Require Import Crypto.Util.Option.
+Require Import Crypto.Util.ListUtil.
+Require Import Coq.Lists.List. (* after SeparationLogic *)
+Import ListNotations.
+
+(* This file contains general-purpose lemmas about other libraries that should
+   eventually be moved to those libraries or to coqutil *)
+
+Section Lists.
+  Context {A : Type}.
+
+  Lemma hd_map {B} (f : A -> B) x l :
+    hd (f x) (map f l) = f (hd x l).
+  Proof. destruct l; reflexivity. Qed.
+
+  Lemma hd_skipn_nth_default (d:A) l i :
+    nth_default d l i = hd d (skipn i l).
+  Proof.
+    revert i; induction l; destruct i; try reflexivity.
+    rewrite nth_default_cons_S, skipn_cons_S. eauto.
+  Qed.
+
+  Lemma firstn_length_firstn n (l : list A) :
+    firstn (length (firstn n l)) l = firstn n l.
+  Proof.
+    revert l; induction n; destruct l;
+      cbn [firstn length]; rewrite ?IHn; reflexivity.
+  Qed.
+
+  Lemma skipn_length_firstn n (l : list A) :
+    skipn (length (firstn n l)) l = skipn n l.
+  Proof.
+    revert l; induction n; destruct l;
+      cbn [skipn firstn length]; rewrite ?IHn; reflexivity.
+  Qed.
+
+  Lemma NoDup_app_iff (l1 l2 : list A) :
+    NoDup (l1 ++ l2) <-> (NoDup l1 /\ NoDup l2
+                          /\ (forall x, In x l1 -> ~ In x l2)
+                          /\ (forall x, In x l2 -> ~ In x l1)).
+  Proof.
+    revert l2; induction l1;
+      repeat match goal with
+             | _ => progress (intros; subst)
+             | _ => progress cbn [In]
+             | _ => rewrite app_nil_l
+             | _ => rewrite <-app_comm_cons
+             | _ => split
+             | H : _ /\ _ |- _ => destruct H
+             | H : _ \/ _ |- _ => destruct H
+             | H: ~ In _ (_ ++ _) |- _ =>
+               rewrite in_app_iff in H;
+                 apply Decidable.not_or in H
+             | H: NoDup (_ ++ _) |- _ =>
+               apply IHl1 in H
+             | H: NoDup (_ :: _) |- _ =>
+               inversion H; clear H; subst
+             | |- ~ (_ \/ _) => intro
+             | |- ~ In _ (_ ++_) =>
+               rewrite in_app_iff
+             | |- NoDup (_ ++ _) => apply IHl1
+             | |- NoDup (_ :: _) => constructor
+             | |- NoDup [] => constructor
+             | H1 : (forall x (H:In x ?l), _),
+                    H2 : In _ ?l |- _ => apply H1 in H2; tauto
+             | H : forall x (_:?a = x \/ _), _ |- _ =>
+               specialize (H a ltac:(tauto)); tauto
+             | _ => solve [eauto]
+             | _ => tauto
+             end.
+  Qed.
+End Lists.
+
+Section Sets.
+  Context {E : Type}.
+
+  Lemma disjoint_union_l_iff (s1 s2 s3 : set E) :
+    disjoint (union s1 s2) s3 <-> disjoint s1 s3 /\ disjoint s2 s3.
+  Proof. firstorder idtac. Qed.
+
+  Lemma disjoint_union_r_iff (s1 s2 s3 : set E) :
+    disjoint s1 (union s2 s3) <-> disjoint s1 s2 /\ disjoint s1 s3.
+  Proof. firstorder idtac. Qed.
+
+  Lemma disjoint_cons (s : set E) x l :
+    disjoint s (of_list (x :: l)) ->
+    disjoint s (of_list l) /\ disjoint s (singleton_set x).
+  Proof. firstorder idtac. Qed.
+
+  Lemma disjoint_singleton_r_iff
+        (x : E) (s : set E)
+        (eq_dec : forall a b : E, {a = b} + {a <> b}):
+    ~ s x <->
+    disjoint s (singleton_set x).
+  Proof.
+    intros. split; [|firstorder idtac].
+    intros. intro y.
+    destruct (eq_dec x y);
+      subst; try firstorder idtac.
+  Qed.
+
+  Lemma disjoint_singleton_singleton
+        (x y : E)
+        (eq_dec : forall a b : E, {a = b} + {a <> b}):
+    y <> x ->
+    disjoint (singleton_set x) (singleton_set y).
+  Proof.
+    intros.
+    apply disjoint_singleton_r_iff;
+      firstorder congruence.
+  Qed.
+
+  Lemma disjoint_sameset (s1 s2 s3 : set E) :
+    sameset s3 s1 ->
+    disjoint s1 s2 ->
+    disjoint s3 s2.
+  Proof. firstorder idtac. Qed.
+
+  Global Instance disjoint_sym : Symmetric (@disjoint E).
+  Proof. firstorder idtac. Defined.
+  Global Instance disjoint_Proper
+    : Proper (sameset ==> sameset ==> iff) (@disjoint E).
+  Proof. firstorder idtac. Defined.
+
+  Global Instance sameset_sym : Symmetric (@sameset E).
+  Proof. firstorder idtac. Defined.
+  Global Instance sameset_trans : Transitive (@sameset E).
+  Proof. firstorder idtac. Defined.
+  Global Instance sameset_ref : Reflexive (@sameset E).
+  Proof. firstorder idtac. Defined.
+
+  Lemma sameset_iff (s1 s2 : set E) :
+    sameset s1 s2 <-> (forall e, s1 e <-> s2 e).
+  Proof. firstorder idtac. Qed.
+
+  Lemma not_union_iff (s1 s2 : set E) x :
+    ~ union s1 s2 x <-> ~ s1 x /\ ~ s2 x.
+  Proof. firstorder idtac. Qed.
+
+  Lemma disjoint_not_in x (l : list E)
+        (eq_dec : forall a b : E, {a = b} + {a <> b}) :
+    ~ In x l ->
+    disjoint (singleton_set x) (of_list l).
+  Proof.
+    intros. symmetry. apply disjoint_singleton_r_iff; eauto.
+  Qed.
+
+  Lemma NoDup_disjoint (l1 l2 : list E)
+        (eq_dec : forall a b : E, {a = b} + {a <> b}) :
+    NoDup (l1 ++ l2) ->
+    disjoint (of_list l1) (of_list l2).
+  Proof.
+    revert l2; induction l1; intros *;
+      rewrite ?app_nil_l, <-?app_comm_cons;
+      [ solve [firstorder idtac] | ].
+    inversion 1; intros; subst.
+    rewrite PropSet.of_list_cons.
+    apply disjoint_union_l_iff; split; eauto.
+    apply disjoint_not_in; eauto.
+    rewrite in_app_iff in *. tauto.
+  Qed.
+End Sets.
+
+Section Maps.
+  Context {key value} {key_eqb}
+          {map : map.map key value}
+          {key_eq_dec :
+             forall x y : key,
+               BoolSpec (x = y) (x <> y) (key_eqb x y)}
+          {map_ok : map.ok map}.
+
+  Lemma only_differ_sym m1 m2 ks :
+    map.only_differ m1 ks m2 ->
+    map.only_differ m2 ks m1.
+  Proof. firstorder congruence. Qed.
+
+  Lemma only_differ_trans m1 m2 m3 ks1 ks2 :
+    map.only_differ m2 ks1 m1 ->
+    map.only_differ m3 ks2 m2 ->
+    map.only_differ m3 (union ks1 ks2) m1.
+  Proof. firstorder congruence. Qed.
+
+  Global Instance Proper_only_differ :
+    Proper (eq ==> sameset ==> eq ==> iff) map.only_differ.
+  Proof. firstorder congruence. Qed.
+
+  Lemma only_differ_put m k v :
+    map.only_differ (map.put m k v) (singleton_set k) m.
+  Proof.
+    cbv [map.only_differ elem_of singleton_set].
+    intro x; destr (key_eqb k x); subst;
+      rewrite ?map.get_put_same, ?map.get_put_diff by congruence;
+      tauto.
+  Qed.
+
+  Lemma putmany_of_list_zip_app_l m ks1 ks2 vs :
+    map.putmany_of_list_zip (ks1 ++ ks2) vs m =
+    Option.bind
+      (map.putmany_of_list_zip
+         ks1 (List.firstn (Datatypes.length ks1) vs) m)
+      (map.putmany_of_list_zip
+         ks2 (List.skipn (Datatypes.length ks1) vs)).
+  Admitted.
+
+  Lemma putmany_of_list_zip_bind_comm m ks1 ks2 vs1 vs2 :
+    Option.bind
+      (map.putmany_of_list_zip ks1 vs1 m)
+      (map.putmany_of_list_zip ks2 vs2) =
+    Option.bind
+      (map.putmany_of_list_zip ks2 vs2 m)
+      (map.putmany_of_list_zip ks1 vs1).
+  Admitted.
+End Maps.
+
+(* These lemmas should be moved to bedrock2, not coqutil *)
+Section Separation.
+  Context `{map_ok : map.ok}
+           {key_eqb : forall H H0 : key, bool}
+           {key_eq_dec :
+              forall x y : key,
+                BoolSpec (x = y) (x <> y) (key_eqb x y)}.
+  Lemma sep_empty_iff (q r : map.rep -> Prop) :
+    sep q r map.empty <-> q map.empty /\ r map.empty.
+  Proof.
+    cbv [sep].
+    repeat match goal with
+           | _ => progress (intros; subst)
+           | H : _ /\ _ |- _ => destruct H
+           | H : exists _, _ |- _ => destruct H
+           | H : _ |- _ => apply map.split_empty in H
+           | _ => rewrite map.split_empty
+           | _ => exists map.empty
+           | _ => tauto
+           | _ => split
+           end.
+  Qed.
+End Separation.
